\documentclass[11pt, oneside]{article} 
\usepackage{geometry}
\geometry{letterpaper} 
\usepackage{graphicx}
	
\usepackage{amssymb}
\usepackage{amsmath}
\usepackage{parskip}
\usepackage{color}
\usepackage{hyperref}

\graphicspath{{/Users/telliott/Dropbox/Github-Math/figures/}}
% \begin{center} \includegraphics [scale=0.4] {gauss3.png} \end{center}

\title{Tangents}
\date{}

\begin{document}
\maketitle
\Large

%[my-super-duper-separator]

\subsection*{parabola}

Suppose we have a parabola and a point not on the parabola, but in the plane and outside of the "cup" of the parabola, such as $(3,5)$.  We seek the equations of tangent lines to the parabola that go through this point.  
\begin{center} \includegraphics [scale=0.4] {para12.png} \end{center}

There will be two of them.  We show just one in the figure.

The lines passing through this point with different slopes $m$ are given by:

\[ (y - y') = m(x - x') \]
Here, let $(x',y')$ be $(3,5)$:

\[ y - 5 = m(x - 3) \]

Since values of $(x,y)$ are both on the line and the parabola $y=x^2$, we can plug in for $y$:
\[ x^2 - 5 = mx - 3m \]
\[ x^2 - mx + (3m - 5) = 0 \]

As before, solutions are given by the quadratic equation.  

Remember here that $m$ is fixed.  We seek values for $(x,y)$ which are both on the line, and on the curve.  For most $m$ there will be two solutions.  But when $m$ is the slope of the tangent line, there is only one $x$ that solves the equation.

The value of the slope $m$ giving a single solution (zero discriminant) is:
\[ (-m)^2 - 4(3m - 5) = 0 \]
\[ m^2 - 12m + 20 = 0 \]

Another quadratic.  We can factor it by eye:
\[ (m - 2)(m - 10) = 0 \]
\[ m = 2, \ \ \ m = 10 \]

We knew the first one already, because the point $(x',y') = (3,5)$ is on the line $y = 2x - 1$.  This is the tangent to the curve at $(1,1)$, which has slope $m = 2$.
\begin{center} \includegraphics [scale=0.50] {para13.png} \end{center}

The original point $(3,5)$ isn't shown.

As mentioned, there is always another solution which we haven't found explicitly and isn't shown on the graph either.  Any vertical line (with infinite slope) passes through only a single point on the parabola.

We ignore this complication.

\subsection*{general solution}
We are given the parabola $y = ax^2$, as well as a general point $(x',y')$, which we suppose is not on the parabola.  Any line through the point $(x',y')$ has the equation:
\[ y - y' = m(x - x') \]
for all points $(x,y)$ on the line.

If one of those points $(x,y)$ is on the line and \emph{also} on the parabola, it must satisfy $y = ax^2$ as well, so:

\[ ax^2 - y' = m(x - x') \]
\[ ax^2 - mx + (mx' - y') = 0 \]

The must be only one value of $x$ which works for a particular $m$, there can be \emph{no other solutions}.  (In general, for a point $(x',y')$ \emph{underneath} the parabola there will be two tangent lines).

Write the quadratic equation to solve for $x$:
\[ x = \frac{m \pm \sqrt{m^2 - 4a(mx' - y')}}{2a} \]

There is a single solution when the discriminant is zero.  Then
\[ x = \frac{m}{2a} \]
\[ m = 2ax \]

At the point $(x,y) = (1,1)$, the slope is equal to $2$, if $y = x^2$.

Go back to the equation for the line
\[ y - y' = m(x - x') \]

and plug in this slope
\[ y - y' = 2ax(x - x') \]

Then for a given $(x',y')$ we can find the two points $(x,y)$ as
\[ ax^2 - y' = 2ax^2 - 2axx' \]
\[ ax^2 - 2ax'x + y' = 0 \]

\[ x = \frac{2ax' \pm \sqrt{(2ax')^2 - 4ay'}}{2a} \]
\[ = x' \pm \sqrt{x'^2 - y'/a} \]

There is one solution when the discriminant is zero:
\[ y' = ax'^2 \]
That's when the given point $(x',y')$ actually was on the curve.

And there are no solutions (in the real numbers) when the discriminant is negative:
\[ x'^2 - y'/a < 0 \]
\[ ax'^2 < y' \]

That is, when the point $(x',y')$ lies in the "cup" of the parabola and $y' > ax'^2$.  Then no tangent line runs through $(x',y')$.

\subsection*{circle}

The tangent to the circle from an exterior point is a bit more complicated than for the parabola, because of the square root in the equation $y = \sqrt{r^2 - x^2}$.  We introduce the subject as follows.

This is a problem I found on Twitter (\#GeometrySnacks).

\begin{center} \includegraphics [scale=0.6] {tangent_prob.png} \end{center}

Assume that the curve is a circle, the enclosing box is a square, and the hypotenuse of the pink triangle is the tangent to the curve at some point $T$ which is not shown explicitly.  The base is bisected at the yellow dot, which we will call $P$.  Since this is a unit circle and $RS$ is bisected, the coordinates of $P$ are $(1/2,-1)$.

Since two tangent lines meet at $P$, it follows that the length of the line segment $PT$ is equal to $RP$, giving an isosceles triangle $\triangle RPT$.  But it is given that the base is bisected, hence another isosceles triangle is $\triangle PST$.

\begin{center} \includegraphics [scale=0.4] {tangent_prob2.png} \end{center}

\subsection*{clever solution}

I worked on this problem and obtained the correct solution, but there is an easier way which I did not see.  Perhaps you will find it, if you try before reading any further.

The key to the short solution is to see that there is \emph{another} pair of tangents in the problem: $QT$ and the vertical from $Q$ to the $x$-axis.  So these two distances are also equal.

It follows that the hypotenuse of $\triangle QPS$ is composed of two segments, one equal to $x$, and one equal to $1 - y$, so the Pythagorean theorem gives

\[ (x + (1 - y))^2 = x^2 + y^2 \]
\[ x^2 + x - xy + x + 1 - y - xy - y + y^2 = x^2 + y^2 \]

Canceling and grouping like terms
\[ 2x - 2xy - 2y + 1  = 0  \]
\[ x + \frac{1}{2} = y(x + 1) \]
\[ y = \frac{x + 1/2}{x + 1} \]

But we are given that $x = 1/2$ so
\[ y = \frac{2}{3} \]

The area is
\[ A = \frac{1}{2} \cdot \frac{1}{2} \cdot \frac{2}{3} =  \frac{1}{6}  \]

\subsection*{tangent to a circle}

In general, if we know the slope of the hypotenuse, we can use that to get the altitude and thus the area of the pink triangle from $\Delta y = \text{slope} \cdot \Delta x$, where $\Delta x$ is half the side of the square.

An easy way to see that is to use the figure below.

\begin{center} \includegraphics [scale=0.5] {tangent_prob3.png} \end{center}

$\angle EFK$ and $\angle DFH$ are complementary, so the right triangles $\triangle EFK$ and $\triangle DFH$ similar.  Therefore $FK/EK$ (slope of the tangent) is equal to $DH/HF$ (radial vector $x,y$).  We need a minus sign to turn $y$ into a length.

Or, we might remember that the product of the slopes of two perpendicular lines, such as the radius and tangent to the circle at that point, is equal to $-1$. 

For a circle centered on the origin, the radius to any point on the circle $T = (x,y)$ has slope $y/x$.  Hence the tangent at $T$ has slope $-x/y$, because the product of slopes must be equal to $-1$.  If the circle is not centered on the origin, there will be a correction factor.

Write the equation of the tangent line in terms of the slope $m$ as
\[ m =  \frac{y - (-1)}{x - 1/2} \]

Using the expression from above for $m$ we have 

\[ -\frac{x}{y} =  \frac{y - (-1)}{x - 1/2} \]
\[ y^2 + y = -x^2 + \frac{1}{2} x \]

Since $x^2 + y^2 = 1$ everywhere on the circle,
\[ y + 1 = \frac{1}{2} x  \]

This is a relationship between the $x$- and $y$- values at $T$, but it is clearly not the equation of the tangent line, since $(1/2,-1)$ is not a solution.  

The trick here is to use the information from the circle \emph{again}:

\[ \sqrt{1 - x^2} = \frac{1}{2} x - 1 \]
\[ 1 - x^2 = \frac{1}{4}x^2 - x + 1 \]
\[ \frac{5}{4}x^2 - x = 0 \]
\[ (\frac{5}{4}x - 1) \cdot x = 0 \]

This has two solutions, $x = 0$ and $x = 4/5$, which are indeed the points of tangency as the following analysis will confirm.

Then $y = \sqrt{1 - x^2} = -3/5$ (the minus sign because this is the fourth quadrant).  So the slope is 
\[ \frac{-x}{y} = \frac{-4/5}{-3/5} = \frac{4}{3} \]

which we confirm by the point-slope form:

\[ m = \frac{-3/5 - (-1)}{4/5 - 1/2} = \frac{2/5}{3/10} = \frac{4}{3} \]

So $\Delta y$ for the pink triangle is one-half that.

\subsection*{tangent from an exterior point}

Here's a somewhat longer general approach.

Place the origin of coordinates at the center of a unit circle $x^2 + y^2 = 1$.  Then the point $P = (1/2,-1)$.  The lower point of tangency is $(0,-1)$.

We can draw a line from $P$ to any point on the circle, label it $(x,y)$.  The slope of the line
is $m$ and the equation of the line is
\[ \frac{y - (-1)}{x - 1/2} = m \]

The key insight is that, for the right value of $m$, the resulting line will be the tangent, and then there will be only one $(x,y)$ which solves the equation above and also lie on the circle.  

Substitute for $y$ from the equation of the circle $y = \sqrt{1 - x^2}$.

\[ \frac{\sqrt{1 - x^2} + 1}{x - \frac{1}{2}} = m \]
\[ \sqrt{1 - x^2} = m(x - \frac{1}{2}) - 1 \]

Square both sides
\[ 1 - x^2 = (mx - \frac{1}{2}m - 1)^2 \]
\[ = m^2 x^2 - \frac{1}{2}m^2x - mx - \frac{1}{2}m^2x +  \frac{1}{4}m^2 + \frac{1}{2}m - mx + \frac{1}{2}m + 1   \]
Cancel the one and combine three pairs of terms
\[ -  x^2 = m^2 x^2 - m^2x - 2mx  +  \frac{1}{4}m^2 + m   \]
Group by powers of $x$:
\[ (1 + m^2)x^2 - (m^2 + 2m)x + (m + \frac{1}{4}m^2)  = 0 \]

This is a quadratic in $x$.  There will be one solution when the discriminant is equal to zero.

\[ (m^2 + 2m)^2 = (4)(1 + m^2)(m + \frac{1}{4}m^2) \]
\[ (m^2 + 2m)^2 = (1 + m^2)(4m + m^2) \]
\[ m^4 + 4m^3 + 4m^2 = 4m + m^2 + 4m^3 + m^4 \]

Luckily, there are two cancellations:
\[ 4m^2 = 4m + m^2 \]
\[ (3m - 4)m = 0 \]

One solution is $m=0$.  We knew that:  the horizontal line through $P$ is the other tangent.  

The solution we want is $m = 4/3$.

Knowing the slope of the tangent line and $\Delta x = 1/2$, we find
\[ \Delta y = \frac{4}{3} \cdot \frac{1}{2} \]
\[ = \frac{2}{3} \]

The area is then
\[ A = \frac{1}{2} \cdot \frac{1}{2} \cdot \frac{2}{3} = \frac{1}{6}  \]

\subsection*{other points}

We have that the slope is $4/3$ and one point on the line is $P=(1/2,-1)$.  

The $y$-intercept $y_0$ is
\[ (-1) = \frac{4}{3} \cdot \frac{1}{2} + y_0 \]

which means that $y_0 = -5/3$ and the equation of the line is
\[ y = \frac{4}{3}x - \frac{5}{3} \]

The $x$-intercept is 
\[ y = 0 = \frac{4}{3}x - \frac{5}{3} \]
\[ x = \frac{5}{4} \]

We check to see that $-y_0/x_0$ gives the correct slope, $\Delta y/\Delta x = 4/3$.

We find the $y$-coordinate of the top of the triangle when $x = 1$ so
\[ y = \frac{4}{3}(1) - \frac{5}{3} = - \frac{1}{3} \]

So the side of the triangle is $-1/3 - (-1) = 2/3$, as we found before.

Last, we want the point on the circle.  We use the original idea that the product of the slopes is $-1$, so the point $(x,y)$ would be $(4,-3)$ except that this needs to be normalized to have a length of $1$.  

That normalization constant is $\sqrt{3^2 + 4^2} = 5$ so finally

\[ T = (\frac{4}{5}, -\frac{3}{5}) \]

This point satisfies the equation of the circle and it lies on the line since
\[ -\frac{3}{5} = \frac{4}{3} \cdot \frac{4}{5} - \frac{5}{3}  \]
\[ -9 = 16 - 25 \]

$\circ$

There are a number of similar 3-4-5 right triangles in the final figure.
\begin{center} \includegraphics [scale=1] {tangent_prob1.png} \end{center}

\subsection*{complete general equation}

The algebra was simplified somewhat above by the fact that the exterior point had coordinates $(1/2,-1)$.  The general case has $(x,y)$ on the circle and we will use $(h,k)$ for the point.  

(We use $(h,k)$ rather than $(x',y')$ because the algebra is so involved.  Normally $(h,k)$ is used for the origin or vertex of a displaced curve, not at the origin.)

The circle can have any radius $r > 0$.

The slope is
\[ m = \frac{y - k}{x - h} \]

and $y = \sqrt{r^2 - x^2}$ so
\[ m(x - h) + k = \sqrt{r^2 - x^2} \]

Square both sides
\[ m^2(x - h)^2 + 2m(x-h)k + k^2 = r^2 - x^2 \]

\[ m^2x^2 - 2m^2xh + m^2h^2 + 2m(x-h)k + k^2 = r^2 - x^2 \]
\[ (m^2 + 1) x^2 - 2m(mh - k) x + m^2h^2 - 2mhk + k^2 - r^2 = 0 \]

There's a repeated term:  $(mh - k)$ in the $x^1$ and$(mh - k)^2$ in the $x^0$ power, but it doesn't help with what comes below because of the extra $1$ at the end.

The discriminant should be zero, since for a given $m$ we want a unique $x$ and $y$ on the circle.
\[ 4m^2(mh - k)^2 = 4(m^2 + 1)(m^2h^2 - 2mhk + k^2 - r^2) \]

This would be a fourth power of $m$ as well as a third (not good), but it works out.  First, cancel the $4$
\[ m^2(mh - k)^2 = (m^2 + 1)(m^2h^2 - 2mhk + k^2 - r^2) \]

The left-hand side is
\[ m^2(m^2h^2 - 2mhk + k^2) = m^4h^2 - 2m^3hk + m^2k^2 \]

The right-hand side is
\[ (m^2 + 1)(m^2h^2 - 2mhk + k^2 - r^2) \]
\[ = m^4h^2 - 2m^3hk + m^2 k^2 - m^2 + m^2h^2 - 2mhk + k^2 - r^2 \]

After canceling the entire left-hand side
\[ 0 = -m^2 + m^2h^2 - 2mhk + k^2 - r^2 \]
\[ (h^2 - 1)m^2  - 2hkm + (k^2 - r^2) = 0 \]

Plugging into the quadratic equation:
\[ \frac{2hk \pm \sqrt{4h^2k^2 - 4(h^2 - 1)(k^2 - r^2)}}{2(h^2 - 1)} \]
\[ \frac{hk \pm \sqrt{h^2k^2 - (h^2 - 1)(k^2 - r^2)}}{(h^2 - 1)} \]
\[ \frac{hk \pm \sqrt{h^2 + k^2 - r^2}}{(h^2 - 1)} \]

This is a general expression for the slope of the tangent to the circle, centered at the origin, from a point $(h,k)$.

Now, $h^2 + k^2$ must be $ \ge r^2$, otherwise there is no real solution.  There is no tangent from an interior point.

In the case of equality, we would have that the slope is 
\[ m = \frac{hk}{h^2 - 1} = \frac{hk}{-k^2} = -\frac{h}{k} \]

The slope of the tangent at a point $(h,k)$ on the circle is $-h/k$.  We already knew this and it's nice to see that it matches.

In this problem we have $k = -1$ so this is just
\[ \frac{-h \pm h}{h^2 - 1} \]

One answer is $h = 0$ so $m=0$.  (Look at the figure again to see why this is correct).

Plugging in $h = -1/2$, the other is
\[ m = \frac{-2(1/2)}{1/4 - 1} = \frac{-1}{-3/4} = \frac{4}{3}  \]

This matches our previous work.

We look at the ellipse in the next chapter

\[ \frac{x^2}{a^2} + \frac{y^2}{b^2} = 1 \]

We will not solve this problem for the ellipse, although you might adapt the approach shown above.  I obtained this expression for $m$:

\[ \frac{hk \pm b \sqrt{-h^2 + k^2/a^2 - b^2/a^2)}}{(h^2 - b^2/a^2)} \]

Another, much simpler possibility, is to just transform the variables to $au = x$ and $bv = y$.

\[ \frac{(au)^2}{a^2} + \frac{(bv)^2}{b^2} = u^2 + v^2 = 1 \]

Now, solve the problem as a circle, and then transform the result back.

\end{document}
